refactor(data/list/sort): simplify proofs

data/list/sort.lean
@@ -87,7 +87,7 @@ section insertion_sort
 
 def ordered_insert (a : α) : list α → list α
 | []       := [a]
-| (b :: l) := if a ≼ b then a :: (b :: l) else b :: ordered_insert l
+| (b :: l) := if a ≼ b then a :: b :: l else b :: ordered_insert l
 
 --@[simp]
 --theorem ordered_insert_nil (a : α) : ordered_insert a [] = [a] := rfl
@@ -109,55 +109,33 @@ parameter [deceqα : decidable_eq α]
 include deceqα
 open perm
 
--- TODO(Jeremy): anonymous type class parameters don't work well
-
-theorem count_ordered_insert_eq (b a : α) : ∀ l, count b (ordered_insert a l) = count b (a :: l)
-| []       := by simp [ordered_insert]
-| (c :: l) := if h : a ≼ c then begin unfold ordered_insert, simp [if_pos, h] end
-              else by simp [ordered_insert, if_neg, h, count_cons', count_ordered_insert_eq]
-
-theorem mem_ordered_insert_iff (b a : α) (l : list α) : b ∈ ordered_insert a l ↔ b ∈ a :: l :=
-begin repeat {rw mem_iff_count_pos}, simp [count_ordered_insert_eq] end
+theorem perm_ordered_insert (a) : ∀ l : list α, ordered_insert a l ~ a :: l
+| []       := perm.refl _
+| (b :: l) := by simp [ordered_insert]; by_cases a ≼ b; simp [h];
+  exact (perm.skip _ (perm_ordered_insert l)).trans (perm.swap _ _ _)
 
 theorem perm_insertion_sort : ∀ l : list α, insertion_sort l ~ l
 | []       := perm.nil
-| (b :: l) := perm_of_forall_count_eq (assume a,
-                by simp [insertion_sort, count_ordered_insert_eq, count_cons',
-                         count_eq_count_of_perm (perm_insertion_sort l) a])
+| (b :: l) := by simp [insertion_sort]; exact
+  (perm_ordered_insert _ _ _).trans (perm.skip b (perm_insertion_sort l))
 
 section total_and_transitive
 variables (totr : total r) (transr : transitive r)
 include totr transr
 
 theorem sorted_ordered_insert (a : α) : ∀ l, sorted r l → sorted r (ordered_insert a l)
-| []       := assume h, sorted_singleton r a
-| (b :: l) :=
-  assume h,
-  have sorted r l, from sorted_of_sorted_cons r h,
-  have h₀ : ∀ c ∈ l, b ≼ c, from forall_mem_rel_of_sorted_cons r h,
-  if h' : a ≼ b then
-    begin
-      simp [ordered_insert, if_pos, h'],
-      exact have ∀ c ∈ b :: l, a ≼ c, from
-        assume c, assume : c ∈ b :: l,
-        or.elim (eq_or_mem_of_mem_cons this)
-          (assume : c = b, this^.symm ▸ ‹a ≼ b›)
-          (assume : c ∈ l, transr ‹a ≼ b› (h₀ _ this)),
-      show sorted r (a :: b :: l), from sorted_cons r h this
-   end
-  else
-    have b ≼ a, from or.resolve_left (totr a b) h',
-    begin
-      simp [ordered_insert, if_neg, ‹¬ a ≼ b›],
-      exact have h₁ : sorted r (ordered_insert r a l), from sorted_ordered_insert l ‹sorted r l›,
-      have h₂ : ∀ c ∈ ordered_insert r a l, b ≼ c, from
-        assume c,
-        assume : c ∈ ordered_insert r a l,
-        have c ∈ a  :: l, from (mem_ordered_insert_iff r c a l)^.mp this,
-        or.elim (eq_or_mem_of_mem_cons this)
-          (assume : c = a, begin rw this, exact ‹b ≼ a› end)
-          (assume : c ∈ l, h₀ c this),
-      show sorted r (b :: ordered_insert r a l), from sorted_cons r h₁ h₂
+| []       h := sorted_singleton r a
+| (b :: l) h := begin
+    simp [ordered_insert]; by_cases a ≼ b with h'; simp [h'],
+    { rw [sorted], refine ⟨h, λ b' bm, _⟩,
+      simp at bm, cases bm with be bm,
+      { subst b', exact h' },
+      { exact transr h' (h.right _ bm) } },
+    { rw [sorted], refine ⟨sorted_ordered_insert l h.left, λ b' bm, _⟩,
+      have bm := mem_of_perm (perm_ordered_insert _ _ _) bm,
+      simp at bm, cases bm with be bm,
+      { subst b', exact (totr _ _).resolve_left h' },
+      { exact h.right _ bm } }
     end
 
 theorem sorted_insert_sort : ∀ l, sorted r (insertion_sort l)
@@ -177,252 +155,141 @@ section merge_sort
 
 def split : list α → list α × list α
 | []            := ([], [])
-| [a]           := ([a], [])
-| (a :: b :: l) := match split l with
-                   | (l₁, l₂) := (a :: l₁, b :: l₂)
-                   end
+| (a :: l) := let (l₁, l₂) := split l in (a :: l₂, l₁)
+attribute [simp] split
 
--- TODO(Jeremy): the cases is needed because the internal split_match gets a pair
+theorem split_cons_of_eq (a : α) {l l₁ l₂ : list α} (h : split l = (l₁, l₂)) :
+  split (a :: l) = (a :: l₂, l₁) :=
+by rw [split, h]; refl
 
-private theorem split_cons_cons_aux (a b : α) (l : list α) :
-  split (a :: b :: l) = match split l with
-                   | (l₁, l₂) := (a :: l₁, b :: l₂)
-                   end := rfl
-
-@[simp]
-theorem split_cons_cons (a b : α) (l : list α) :
-  split (a :: b :: l) = (a :: (split l).1, b :: (split l).2) :=
-begin rw [split_cons_cons_aux], cases split l, reflexivity end
-
-theorem length_split_fst_le : ∀ l : list α, length ((split l).1) ≤ length l
-| []            := nat.le_refl 0
-| [a]           := nat.le_refl 1
-| (a :: b :: l) := begin
-                     simp [split_cons_cons, -add_comm],
-                     exact nat.succ_le_succ (nat.le_succ_of_le (length_split_fst_le l))
-                   end
-
-theorem length_split_snd_le : ∀ l : list α, length ((split l).2) ≤ length l
-| []            := nat.le_refl 0
-| [a]           := nat.zero_le 1
-| (a :: b :: l) := begin
-                     simp [-add_comm],
-                     transitivity,
-                     { apply add_le_add_right (length_split_snd_le l) },
-                     simp [nat.one_add, nat.le_succ]
-                   end
-
-theorem length_split_cons_cons_fst_lt (a b : α) (l : list α) :
-  length (split (a :: b :: l)).1 < length (a :: b :: l) :=
-begin
-  simp [-add_comm],
-  exact add_lt_add_of_le_of_lt (length_split_fst_le l) (nat.le_refl _)
+theorem length_split_le : ∀ {l l₁ l₂ : list α},
+  split l = (l₁, l₂) → length l₁ ≤ length l ∧ length l₂ ≤ length l
+| []     ._  ._  rfl := ⟨nat.le_refl 0, nat.le_refl 0⟩
+| (a::l) l₁' l₂' h   := begin
+  ginduction split l with e l₁ l₂,
+  injection (split_cons_of_eq _ e).symm.trans h,
+  subst l₁', subst l₂',
+  cases length_split_le e with h₁ h₂,
+  exact ⟨nat.succ_le_succ h₂, nat.le_succ_of_le h₁⟩
 end
 
-theorem length_split_cons_cons_snd_lt (a b : α) (l : list α) :
-  length (split (a :: b :: l)).2 < length (a :: b :: l) :=
+theorem length_split_lt {a b} {l l₁ l₂ : list α} (h : split (a::b::l) = (l₁, l₂)) :
+  length l₁ < length (a::b::l) ∧ length l₂ < length (a::b::l) :=
 begin
-  simp [-add_comm],
-  exact add_lt_add_of_le_of_lt (length_split_snd_le l) (nat.le_refl _)
+  ginduction split l with e l₁' l₂',
+  injection (split_cons_of_eq _ (split_cons_of_eq _ e)).symm.trans h,
+  subst l₁, subst l₂,
+  cases length_split_le e with h₁ h₂,
+  exact ⟨nat.succ_le_succ (nat.succ_le_succ h₁), nat.succ_le_succ (nat.succ_le_succ h₂)⟩
 end
 
--- Do the well-founded recursion by hand, until the function definition system supports it.
+theorem perm_split : ∀ {l l₁ l₂ : list α}, split l = (l₁, l₂) → l ~ l₁ ++ l₂
+| []     ._  ._  rfl := perm.refl _
+| (a::l) l₁' l₂' h   := begin
+  ginduction split l with e l₁ l₂,
+  injection (split_cons_of_eq _ e).symm.trans h,
+  subst l₁', subst l₂',
+  exact perm.skip a ((perm_split e).trans perm.perm_app_comm),
+end
 
-private def merge.F :
-  Π p : list α × list α,
-      (Π p₁ : list α × list α, length p₁.1 + length p₁.2 < length p.1 + length p.2 → list α) →
-    list α
-| ([], l)           f := l
-| (a :: l, [])      f := a :: l
-| (a :: l, b :: l') f := if a ≼ b then
-                           a :: f (l, b :: l') begin simp [-add_comm], apply nat.le_refl end
-                         else
-                           b :: f (a :: l, l') begin apply nat.le_refl end
+def merge : list α → list α → list α
+| []       l'        := l'
+| l        []        := l
+| (a :: l) (b :: l') := if a ≼ b then a :: merge l (b :: l') else b :: merge (a :: l) l'
 
-def merge := well_founded.fix (inv_image.wf _ nat.lt_wf) merge.F
+include r
+def merge_sort : list α → list α
+| []        := []
+| [a]       := [a]
+| (a::b::l) := begin
+  ginduction split (a::b::l) with e l₁ l₂,
+  cases length_split_lt e with h₁ h₂,
+  exact merge r (merge_sort l₁) (merge_sort l₂)
+end
+using_well_founded {
+  rel_tac := λ_ _, `[exact ⟨_, inv_image.wf length nat.lt_wf⟩],
+  dec_tac := tactic.assumption }
 
-theorem merge.def (p : list α × list α) : merge p = merge.F p (λ p h, merge p) :=
-well_founded.fix_eq (inv_image.wf _ nat.lt_wf) merge.F p
-
-@[simp]
-theorem merge.equations.eq_1 (l : list α) : merge ([], l) = l :=
-begin rw merge.def, reflexivity end
-
-@[simp]
-theorem merge.equations.eq_2 (a : α) (l : list α) : merge (a :: l, []) = a :: l :=
-begin rw merge.def, reflexivity end
-
-@[simp]
-theorem merge.equations.eq_3 (a b : α) (l l' : list α) :
-  merge (a :: l, b :: l') = if a ≼ b then
-                             a :: merge (l, b :: l')
-                           else
-                             b :: merge (a :: l, l') :=
-begin rw merge.def, reflexivity end
-
-private def merge_sort.F :
-  Π l : list α, (Π l₁ : list α, length l₁ < length l → list α) → list α
-| []            f := []
-| [a]           f := [a]
-| (a :: b :: l) f := let p  := split (a :: b :: l),
-                         l₁ := f p.1 (length_split_cons_cons_fst_lt a b l),
-                         l₂ := f p.2 (length_split_cons_cons_snd_lt a b l) in
-                     merge (l₁, l₂)
-
-def merge_sort := well_founded.fix (inv_image.wf _ nat.lt_wf) merge_sort.F
-
-theorem merge_sort.def (l : list α) : merge_sort l = merge_sort.F l (λ l h, merge_sort l) :=
-well_founded.fix_eq (inv_image.wf _ nat.lt_wf) merge_sort.F l
-
-@[simp]
-theorem merge_sort.equations.eq_1 : merge_sort [] = [] :=
-begin rw merge_sort.def, reflexivity end
-
-@[simp]
-theorem merge_sort.equations.eq_2 (a : α) : merge_sort [a] = [a] :=
-begin rw merge_sort.def, reflexivity end
-
-@[simp]
-theorem merge_sort.equations.eq_3 (a b : α) (l : list α) :
-  merge_sort (a :: b :: l) = let p := split (a :: b :: l) in
-                             merge (merge_sort p.1, merge_sort p.2) :=
-begin rw merge_sort.def, reflexivity end
+theorem merge_sort_cons_cons {a b} {l l₁ l₂ : list α}
+  (h : split (a::b::l) = (l₁, l₂)) :
+  merge_sort (a::b::l) = merge (merge_sort l₁) (merge_sort l₂) :=
+begin
+  simp [merge_sort, h], dsimp,
+  have : ∀ (L : list α) h1, @@and.rec
+    (λ a a (_ : length l₁ < length l + 1 + 1 ∧
+      length l₂ < length l + 1 + 1), L) h1 h1 = L,
+  { intros, cases h1, refl },
+  apply this
+end
 
 section correctness
 parameter [deceqα : decidable_eq α]
 include deceqα
 
-theorem count_split (a : α) : ∀ l : list α, count a (split l).1 + count a (split l).2 = count a l
-| []            := rfl
-| [a]           := rfl
-| (a :: b :: l) := begin simp [count_cons'], rw [←count_split l], simp end
+theorem perm_merge : ∀ (l l' : list α), merge l l' ~ l ++ l'
+| []       []        := perm.nil
+| []       (b :: l') := by simp [merge]
+| (a :: l) []        := by simp [merge]
+| (a :: l) (b :: l') := by simp [merge]; by_cases a ≼ b; simp [h];
+  [exact perm.skip _ (perm_merge _ _),
+   exact (perm.skip _ (perm_merge _ _)).trans
+     (perm.trans (perm.swap _ _ _) (perm.skip _ (perm.perm_middle _ _ _)))]
 
-private def count_merge.F (c : α) :
-  Π p : list α × list α,
-      (Π p₁ : list α × list α, length p₁.1 + length p₁.2 < length p.1 + length p.2 →
-        count c (merge p₁) = count c p₁.1 + count c p₁.2) →
-    count c (merge p) = count c p.1 + count c p.2
-| ([], l)            f := by simp
-| (a :: l, [])       f := by simp
-| (a :: l, b :: l')  f := if h : a ≼ b then
-                            begin
-                              have hrec := f (l, b :: l') begin simp [-add_comm], apply nat.le_refl end,
-                              simp [if_pos, h, count_cons', hrec]
-                            end
-                          else
-                            begin
-                              have hrec := f (a :: l, l') begin apply nat.le_refl end,
-                              simp [if_neg, h, count_cons', hrec]
-                            end
-
-theorem count_merge (c : α) :
-  ∀ p : list α × list α, count c (merge p) = count c p.1 + count c p.2 :=
-well_founded.fix (inv_image.wf _ nat.lt_wf) (count_merge.F c)
-
-theorem mem_merge_iff (a : α) (p : list α × list α) : a ∈ merge p ↔ a ∈ p.1 ∨ a ∈ p.2 :=
-begin repeat { rw mem_iff_count_pos }, simp [count_merge, nat.add_pos_iff_pos_or_pos] end
-
-private def perm_merge_sort.F :
-  Π l : list α, (Π l₁ : list α, length l₁ < length l → merge_sort l₁ ~ l₁) →
-    merge_sort l ~ l
-| []  f           := by simp; exact perm.refl _
-| [a] f           := by simp; exact perm.refl _
-| (a :: b :: l) f :=
-  perm.perm_of_forall_count_eq
-  begin
-    intro c,
-    let hrec₁ := perm.count_eq_count_of_perm (f _ (length_split_cons_cons_fst_lt a b l)) c,
-    let hrec₂ := perm.count_eq_count_of_perm (f _ (length_split_cons_cons_snd_lt a b l)) c,
-    simp at hrec₁,
-    simp at hrec₂,
-    simp [hrec₁, hrec₂, count_merge, count_split, count_cons']
-  end
-
-theorem perm_merge_sort : ∀ l : list α, merge_sort l ~ l :=
-well_founded.fix (inv_image.wf _ nat.lt_wf) perm_merge_sort.F
+theorem perm_merge_sort : ∀ l : list α, merge_sort l ~ l
+| []        := perm.refl _
+| [a]       := perm.refl _
+| (a::b::l) := begin
+  ginduction split (a::b::l) with e l₁ l₂,
+  cases length_split_lt e with h₁ h₂,
+  rw [merge_sort_cons_cons r e],
+  apply (perm_merge r _ _).trans,
+  exact (perm.perm_app (perm_merge_sort l₁) (perm_merge_sort l₂)).trans (perm_split e).symm
+end
+using_well_founded {
+  rel_tac := λ_ _, `[exact ⟨_, inv_image.wf length nat.lt_wf⟩],
+  dec_tac := tactic.assumption }
 
 section total_and_transitive
 variables (totr : total r) (transr : transitive r)
 include totr transr
 
-private def sorted_merge.F :
-  Π p : list α × list α,
-      (Π p₁ : list α × list α, length p₁.1 + length p₁.2 < length p.1 + length p.2 →
-        (sorted r p₁.1 → sorted r p₁.2 → sorted r (merge p₁))) →
-    sorted r p.1 → sorted r p.2 → sorted r (merge p)
-| ([], l)           f h₁ h₂ := begin simp, exact h₂ end
-| (a :: l, [])      f h₁ h₂ := begin simp, exact h₁ end
-| (a :: l, b :: l') f h₁ h₂ :=
-  have sorted r l, from sorted_of_sorted_cons r h₁,
-  have sorted r l', from sorted_of_sorted_cons r h₂,
-  have h₁₀ : ∀ c ∈ l, a ≼ c, from forall_mem_rel_of_sorted_cons r h₁,
-  have h₂₀ : ∀ c ∈ l', b ≼ c, from forall_mem_rel_of_sorted_cons r h₂,
-  if h : a ≼ b then
-    begin
-      have hrec := f (l, b :: l') begin simp [-add_comm], apply nat.le_refl end,
-      simp [if_pos, h],
-      exact have h₃ : sorted r (merge r (l, b :: l')), from hrec ‹sorted r l› h₂,
-      have h₄ : ∀ c ∈ merge r (l, b :: l'), a ≼ c,
-      begin
-        intros c hc,
-        rw mem_merge_iff at hc,
-        exact or.elim hc
-          (assume : c ∈ l, show a ≼ c, from h₁₀ c this)
-          (assume : c ∈ b :: l',
-            or.elim (eq_or_mem_of_mem_cons this)
-              (assume : c = b, show a ≼ c, from this^.symm ▸ ‹a ≼ b›)
-              (assume : c ∈ l', show a ≼ c, from transr ‹a ≼ b› (h₂₀ c this)))
-      end,
-      show sorted r (a :: merge r (l, b :: l')), from sorted_cons r h₃ h₄
-    end
-  else
-    have h' : b ≼ a, from or.resolve_left (totr a b) h,
-    begin
-      have hrec := f (a :: l, l') begin apply nat.le_refl end,
-      simp [if_neg, h],
-      exact have h₃ : sorted r (merge r (a :: l, l')), from hrec h₁ ‹sorted r l'›,
-      have h₄ : ∀ c ∈ merge r (a :: l, l'), b ≼ c,
-      begin
-        intros c hc,
-        rw mem_merge_iff at hc,
-        exact or.elim hc
-          (assume : c ∈ a :: l,
-            or.elim (eq_or_mem_of_mem_cons this)
-              (assume : c = a, show b ≼ c, from this^.symm ▸ ‹b ≼ a›)
-              (assume : c ∈ l, show b ≼ c, from transr ‹b ≼ a› (h₁₀ c this)))
-          (assume : c ∈ l', show b ≼ c, from h₂₀ c this)
-      end,
-      show sorted r (b :: merge r (a :: l, l')), from sorted_cons r h₃ h₄
-    end
+theorem sorted_merge : ∀ {l l' : list α}, sorted r l → sorted r l' → sorted r (merge l l')
+| []       []        h₁ h₂ := trivial
+| []       (b :: l') h₁ h₂ := by simp [merge]; exact h₂
+| (a :: l) []        h₁ h₂ := by simp [merge]; exact h₁
+| (a :: l) (b :: l') h₁ h₂ := begin
+  simp [merge]; by_cases a ≼ b; simp [h],
+  { refine ⟨sorted_merge h₁.left h₂, λ b' bm, _⟩,
+    have bm := perm.mem_of_perm (perm_merge _ _ _) bm,
+    simp at bm,
+    cases bm with be bm,
+    { subst b', assumption },
+    cases bm with bl bl',
+    { exact h₁.right _ bl },
+    { exact transr h (h₂.right _ bl') } },
+  { refine ⟨sorted_merge h₁ h₂.left, λ b' bm, _⟩,
+    have bm := perm.mem_of_perm (perm_merge _ _ _) bm,
+    simp at bm,
+    have ba : b ≼ a := (totr _ _).resolve_left h,
+    cases bm with be bm,
+    { subst b', assumption },
+    cases bm with bl bl',
+    { exact transr ba (h₁.right _ bl) },
+    { exact h₂.right _ bl' } }
+end
 
-theorem sorted_merge : Π {p : list α × list α},
-  sorted r p.1 → sorted r p.2 → sorted r (merge p) :=
-well_founded.fix (inv_image.wf _ nat.lt_wf) (sorted_merge.F totr transr)
-
-/- elaboration of sorted_merge_sort.F takes forever
-private def sorted_merge_sort.F :
-  Π l : list α, (Π l₁ : list α, length l₁ < length l → sorted r (merge_sort l₁)) →
-    sorted r (merge_sort l)
-| []            f := by simp; exact sorted_nil r
-| [a]           f := by simp; exact sorted_singleton r a
-| (a :: b :: l) f :=
-  begin
-    simp,
-    apply sorted_merge r totr transr,
-    -- this should be handled by the simplifier, i.e. cancel out +1 and rewrite _ < _ + 1 to _ <= _
-    { dsimp,
-      apply f,
-      show length (split l)^.fst + (1 + 0) < length l + (1 + 1),
-        exact add_lt_add_of_le_of_lt (length_split_fst_le l) (add_lt_add_of_le_of_lt (le_refl 1) zero_lt_one) },
-    { dsimp,
-      apply f,
-      show length (split l)^.snd + (1 + 0) < length l + (1 + 1),
-        exact add_lt_add_of_le_of_lt (length_split_snd_le l) (add_lt_add_of_le_of_lt (le_refl 1) zero_lt_one) }
-  end
-
-theorem sorted_merge_sort : ∀ l : list α, sorted r (merge_sort l) :=
-well_founded.fix (inv_image.wf _ nat.lt_wf) (sorted_merge_sort.F totr transr)
--/
+theorem sorted_merge_sort : ∀ l : list α, sorted r (merge_sort l)
+| []        := sorted_nil _
+| [a]       := sorted_singleton _ _
+| (a::b::l) := begin
+  ginduction split (a::b::l) with e l₁ l₂,
+  cases length_split_lt e with h₁ h₂,
+  rw [merge_sort_cons_cons r e],
+  exact sorted_merge r totr transr (sorted_merge_sort l₁) (sorted_merge_sort l₂)
+end
+using_well_founded {
+  rel_tac := λ_ _, `[exact ⟨_, inv_image.wf length nat.lt_wf⟩],
+  dec_tac := tactic.assumption }
 
 end total_and_transitive
 end correctness
@@ -431,8 +298,8 @@ end sort
 
 /- try them out! -/
 
---vm_eval insertion_sort (λ m n : ℕ, m ≤ n) [5, 27, 221, 95, 17, 43, 7, 2, 98, 567, 23, 12]
+--#eval insertion_sort (λ m n : ℕ, m ≤ n) [5, 27, 221, 95, 17, 43, 7, 2, 98, 567, 23, 12]
 
---vm_eval merge_sort     (λ m n : ℕ, m ≤ n) [5, 27, 221, 95, 17, 43, 7, 2, 98, 567, 23, 12]
+--#eval merge_sort     (λ m n : ℕ, m ≤ n) [5, 27, 221, 95, 17, 43, 7, 2, 98, 567, 23, 12]
 
 end list
